theories/RenameApartToPart.v
@@ -65,6 +65,21 @@ Proof.
   eapply even_add; eauto. eapply even_mult2.
 Qed.
 
+Lemma even_fast_update_even E fi (s:set nat) t
+      (Len:❬to_list s❭ = ❬t❭)
+  : forall x : nat,
+    x \In s ->
+    even_inf_subset ((E [to_list s <-- fst (fresh_list FG_even_fast fi t)]) x).
+Proof.
+  intros.
+  rewrite <- of_list_3 in H.
+  eapply (update_with_list_lookup_in_list E _ (fst (fresh_list FG_even_fast fi t))) in H; dcr.
+    + rewrite H2.
+      eapply even_fast_list_even.
+      eapply get_in_of_list; eauto.
+    + rewrite fresh_list_len; eauto using FGS_even_fast.
+Qed.
+
 Lemma rename_to_subset_even s
   : For_all (inf_subset_P even_inf_subset)
             (occurVars (fst (rename_apart_to_part FGS_even_fast s))).
@@ -74,10 +89,6 @@ Proof.
   - intros. eapply FG_even_fast_inf_subset.
   - intros.
     eapply even_fast_list_even; eauto.
-  - intros. rewrite <- of_list_3 in H.
-    eapply (update_with_list_lookup_in_list id _ (fst (fresh_list FG_even_fast (empty_domain FG_even_fast) (to_list (freeVars s))))) in H; dcr.
-    + rewrite H2.
-      eapply even_fast_list_even.
-      eapply get_in_of_list; eauto.
-    + rewrite fresh_list_len; eauto using FGS_even_fast.
+  - intros.
+    eapply even_fast_update_even; eauto.
 Qed.
